src/simple-proof/proof/GeneralToTight.v
@@ -18,86 +18,84 @@ Require Import InvertibleTypes.
     This lemma corresponds to Lemma 3.5 in the paper.
 
     [inert G]                    #<br>#
-    [G ⊢## x: {A: S..U}]        #<br>#
+    [G @@ S ⊢## x: {A: S..U}]        #<br>#
     [――――――――――――――――――――――――――――]   #<br>#
-    [exists T. G ⊢## x: {A: T..T}]   #<br>#
-    [G ⊢# T <: U]               #<br>#
-    [G ⊢# S <: T]                    *)
-Lemma sel_premise: forall G x A S U,
+    [exists T. G @@ S ⊢## x: {A: T..T}]   #<br>#
+    [G @@ S ⊢# T <: U]               #<br>#
+    [G @@ S ⊢# S <: T]                    *)
+Lemma sel_premise: forall G S x A U V,
   inert G ->
-  G ⊢## x : typ_rcd (dec_typ A S U) ->
+  G @@ S ⊢## x : typ_rcd (dec_typ A U V) ->
   exists T,
-    G ⊢! trm_var (avar_f x) : typ_rcd (dec_typ A T T) /\
-    G ⊢# T <: U /\
-    G ⊢# S <: T.
+    G @@ S ⊢! trm_var (avar_f x) : typ_rcd (dec_typ A T T) /\
+    G @@ S ⊢# T <: V /\
+    G @@ S ⊢# U <: T.
 Proof.
   introv HG Hinv.
   dependent induction Hinv.
   - lets Hp: (precise_dec_typ_inv HG H). subst.
-    exists U. split*.
+    exists; split*.
   - specialize (IHHinv A T U0 HG eq_refl).
-    destruct IHHinv as [V [Hx [Hs1 Hs2]]].
-    exists V. split*.
+    destruct IHHinv as [? [Hx [Hs1 Hs2]]].
+    exists; split*.
 Qed.
 
 (** * Sel-<: Replacement
     This lemma corresponds to Lemma 3.4 in the paper.
 
     [inert G]              #<br>#
-    [G ⊢# x: {A: S..U}]   #<br>#
+    [G @@ S ⊢# x: {A: S..U}]   #<br>#
     [――――――――――――――――――――――]   #<br>#
-    [G ⊢# x.A <: U]       #<br>#
-    [G ⊢# S <: x.A]            *)
-Lemma sel_replacement: forall G x A S U,
+    [G @@ S ⊢# x.A <: U]       #<br>#
+    [G @@ S ⊢# S <: x.A]            *)
+Lemma sel_replacement: forall G S x A T U,
     inert G ->
-    G ⊢# trm_var (avar_f x) : typ_rcd (dec_typ A S U) ->
-    (G ⊢# typ_sel (avar_f x) A <: U /\
-     G ⊢# S <: typ_sel (avar_f x) A).
+    G @@ S ⊢# trm_var (avar_f x) : typ_rcd (dec_typ A T U) ->
+    (G @@ S ⊢# typ_sel (avar_f x) A <: U /\
+     G @@ S ⊢# T <: typ_sel (avar_f x) A).
 Proof.
   introv HG Hty.
   pose proof (tight_to_invertible HG Hty) as Hinv.
-  pose proof (sel_premise HG Hinv) as [T [Ht [Hs1 Hs2]]].
-  split.
-  - apply subtyp_sel1_t in Ht. apply subtyp_trans_t with (T:=T); auto.
-  - apply subtyp_sel2_t in Ht. apply subtyp_trans_t with (T:=T); auto.
+  pose proof (sel_premise HG Hinv) as [? [Ht [Hs1 Hs2]]].
+  split; eauto using subtyp_trans_t, subtyp_sel1_t, subtyp_sel2_t.
 Qed.
 
-(** * General to Tight [⊢ to ⊢#] *)
+(** * General to Tight [⊢ to @@ S ⊢#] *)
 (** The following lemma corresponds to Theorem 3.3 in the paper.
     It says that in an inert environment, general typing ([ty_trm] [⊢]) can
     be reduced to tight typing ([ty_trm_t] [⊢#]).
     The proof is by mutual induction on the typing and subtyping judgements.
 
     [inert G]           #<br>#
-    [G ⊢ t: T]          #<br>#
+    [G @@ S ⊢ t: T]          #<br>#
     [――――――――――――――]    #<br>#
-    [G ⊢# t: T] #<br># #<br>#
+    [G @@ S ⊢# t: T] #<br># #<br>#
 
     and                 #<br># #<br>#
     [inert G]           #<br>#
-    [G ⊢ S <: U]        #<br>#
+    [G @@ S ⊢ S <: U]        #<br>#
     [――――――――――――――――]  #<br>#
-    [G ⊢# S <: U]         *)
+    [G @@ S ⊢# S <: U]         *)
 Lemma general_to_tight: forall G0,
   inert G0 ->
-  (forall G t T,
-     G ⊢ t : T ->
+  (forall G S t T,
+     G @@ S ⊢ t : T ->
      G = G0 ->
-     G ⊢# t : T) /\
-  (forall G S U,
-     G ⊢ S <: U ->
+     G @@ S ⊢# t : T) /\
+  (forall G S T U,
+     G @@ S ⊢ T <: U ->
      G = G0 ->
-     G ⊢# S <: U).
+     G @@ S ⊢# T <: U).
 Proof.
   intros G0 HG.
   apply ts_mutind; intros; subst; try solve [eapply sel_replacement; auto]; eauto.
 Qed.
 
 (** The general-to-tight lemma, formulated for term typing. *)
-Lemma general_to_tight_typing: forall G t T,
+Lemma general_to_tight_typing: forall G S t T,
   inert G ->
-  G ⊢ t : T ->
-  G ⊢# t : T.
+  G @@ S ⊢ t : T ->
+  G @@ S ⊢# t : T.
 Proof.
   intros. apply* general_to_tight.
 Qed.
