src/simple-proof/proof/TightTypes.v
@@ -15,10 +15,10 @@ Require Import PreciseTypes.
 
 (** * Tight typing [G |-# t: T] *)
 
-Reserved Notation "G '⊢#' t ':' T" (at level 40, t at level 59).
-Reserved Notation "G '⊢#' T '<:' U" (at level 40, T at level 59).
+Reserved Notation "G '@@' S '⊢#' t ':' T" (at level 40, t at level 59).
+Reserved Notation "G '@@' S '⊢#' T '<:' U" (at level 40, T at level 59).
 
-(** *** Tight term typing [G ⊢# t: T] *)
+(** *** Tight term typing [G @@ S ⊢# t: T] *)
 (** Tight typing is very similar to general typing, and could be obtained by replacing
     all occurrences of [⊢] with [⊢#], except for the following:
     - in the type selection subtyping rules Sel-<: and <:-Sel ([subtyp_sel1] and [subtyp_sel2]),
@@ -26,175 +26,192 @@ Reserved Notation "G '⊢#' T '<:' U" (at level 40, T at level 59).
     - whenever a typing judgement in a premise extends the environment (for example, [ty_all_intro_t]),
       it is typed under general typing [⊢] and not tight typing [⊢#]. *)
 
-Inductive ty_trm_t : ctx -> trm -> typ -> Prop :=
+Inductive ty_trm_t : ctx -> sigma -> trm -> typ -> Prop :=
 
 (** [G(x) = T]   #<br>#
     [――――――――――] #<br>#
-    [G ⊢# x: T]  *)
-| ty_var_t : forall G x T,
+    [G @@ S ⊢# x: T]  *)
+| ty_var_t : forall G S x T,
     binds x T G ->
-    G ⊢# trm_var (avar_f x) : T
+    G @@ S ⊢# trm_var (avar_f x) : T
 
-(** [G, x: T ⊢ t^x: U^x]       #<br>#
+| ty_loc : forall G S l T,
+    binds l T S ->
+    G @@ S ⊢# trm_val (val_loc l) : (typ_ref T)
+
+(** [G, x: T @@ S ⊢ t^x: U^x]       #<br>#
     [x fresh]                  #<br>#
     [――――――――――――――――――――――――] #<br>#
-    [G ⊢# lambda(T)t: forall(T)U]     *)
-| ty_all_intro_t : forall L G T t U,
+    [G @@ S ⊢# lambda(T)t: forall(T)U]     *)
+| ty_all_intro_t : forall L G S T t U,
     (forall x, x \notin L ->
-      G & x ~ T ⊢ open_trm x t : open_typ x U) ->
-    G ⊢# trm_val (val_lambda T t) : typ_all T U
+      G & x ~ T @@ S ⊢ open_trm x t : open_typ x U) ->
+    G @@ S ⊢# trm_val (val_lambda T t) : typ_all T U
 
-(** [G ⊢# x: forall(S)T] #<br>#
-    [G ⊢# z: S]     #<br>#
+(** [G @@ S ⊢# x: forall(S)T] #<br>#
+    [G @@ S ⊢# z: S]     #<br>#
     [――――――――――――――] #<br>#
-    [G ⊢# x z: T^z]     *)
-| ty_all_elim_t : forall G x z S T,
-    G ⊢# trm_var (avar_f x) : typ_all S T ->
-    G ⊢# trm_var (avar_f z) : S ->
-    G ⊢# trm_app (avar_f x) (avar_f z) : open_typ z T
+    [G @@ S ⊢# x z: T^z]     *)
+| ty_all_elim_t : forall G S x z T U,
+    G @@ S ⊢# trm_var (avar_f x) : typ_all T U ->
+    G @@ S ⊢# trm_var (avar_f z) : T ->
+    G @@ S ⊢# trm_app (avar_f x) (avar_f z) : open_typ z U
 
-(** [G, x: T^x ⊢ ds^x :: T^x]    #<br>#
+(** [G, x: T^x @@ S ⊢ ds^x :: T^x]    #<br>#
     [x fresh]                    #<br>#
     [―――――――――――――――――――――――]    #<br>#
-    [G ⊢# nu(T)ds :: mu(T)]         *)
-| ty_new_intro_t : forall L G T ds,
+    [G @@ S ⊢# nu(T)ds :: mu(T)]         *)
+| ty_new_intro_t : forall L G S T ds,
     (forall x, x \notin L ->
-      G & (x ~ open_typ x T) /- open_defs x ds :: open_typ x T) ->
-    G ⊢# trm_val (val_new T ds) : typ_bnd T
+      G & (x ~ open_typ x T) @@ S /- open_defs x ds :: open_typ x T) ->
+    G @@ S ⊢# trm_val (val_new T ds) : typ_bnd T
 
-(** [G ⊢# x: {a: T}] #<br>#
+(** [G @@ S ⊢# x: {a: T}] #<br>#
     [―――――――――――――――] #<br>#
-    [G ⊢# x.a: T]        *)
-| ty_new_elim_t : forall G x a T,
-    G ⊢# trm_var (avar_f x) : typ_rcd (dec_trm a T) ->
-    G ⊢# trm_sel (avar_f x) a : T
+    [G @@ S ⊢# x.a: T]        *)
+| ty_new_elim_t : forall G S x a T,
+    G @@ S ⊢# trm_var (avar_f x) : typ_rcd (dec_trm a T) ->
+    G @@ S ⊢# trm_sel (avar_f x) a : T
 
-(** [G ⊢# t: T]             #<br>#
-    [G, x: T ⊢ u^x: U]       #<br>#
+(** [G @@ S ⊢# t: T]             #<br>#
+    [G, x: T @@ S ⊢ u^x: U]       #<br>#
     [x fresh]                #<br>#
     [――――――――――――――――]       #<br>#
-    [G ⊢# let t in u: U]        *)
-| ty_let_t : forall L G t u T U,
-    G ⊢# t : T ->
+    [G @@ S ⊢# let t in u: U]        *)
+| ty_let_t : forall L G S t u T U,
+    G @@ S ⊢# t : T ->
     (forall x, x \notin L ->
-      G & x ~ T ⊢ open_trm x u : U) ->
-    G ⊢# trm_let t u : U
+      G & x ~ T @@ S ⊢ open_trm x u : U) ->
+    G @@ S ⊢# trm_let t u : U
 
-(** [G ⊢# x: T^x]   #<br>#
+(** [G @@ S ⊢# x: T^x]   #<br>#
     [――――――――――――――] #<br>#
-    [G ⊢# x: mu(T)] *)
-| ty_rec_intro_t : forall G x T,
-    G ⊢# trm_var (avar_f x) : open_typ x T ->
-    G ⊢# trm_var (avar_f x) : typ_bnd T
+    [G @@ S ⊢# x: mu(T)] *)
+| ty_rec_intro_t : forall G S x T,
+    G @@ S ⊢# trm_var (avar_f x) : open_typ x T ->
+    G @@ S ⊢# trm_var (avar_f x) : typ_bnd T
 
-(** [G ⊢# x: mu(T)] #<br>#
+(** [G @@ S ⊢# x: mu(T)] #<br>#
     [――――――――――――――] #<br>#
-    [G ⊢# x: T^x]       *)
-| ty_rec_elim_t : forall G x T,
-    G ⊢# trm_var (avar_f x) : typ_bnd T ->
-    G ⊢# trm_var (avar_f x) : open_typ x T
+    [G @@ S ⊢# x: T^x]       *)
+| ty_rec_elim_t : forall G S x T,
+    G @@ S ⊢# trm_var (avar_f x) : typ_bnd T ->
+    G @@ S ⊢# trm_var (avar_f x) : open_typ x T
 
-(** [G ⊢# x: T]      #<br>#
-    [G ⊢# x: U]      #<br>#
+(** [G @@ S ⊢# x: T]      #<br>#
+    [G @@ S ⊢# x: U]      #<br>#
     [―――――――――――――]   #<br>#
-    [G ⊢# x: T /\ U]      *)
-| ty_and_intro_t : forall G x T U,
-    G ⊢# trm_var (avar_f x) : T ->
-    G ⊢# trm_var (avar_f x) : U ->
-    G ⊢# trm_var (avar_f x) : typ_and T U
+    [G @@ S ⊢# x: T /\ U]      *)
+| ty_and_intro_t : forall G S x T U,
+    G @@ S ⊢# trm_var (avar_f x) : T ->
+    G @@ S ⊢# trm_var (avar_f x) : U ->
+    G @@ S ⊢# trm_var (avar_f x) : typ_and T U
 
-(** [G ⊢# t: T]    #<br>#
-    [G ⊢# T <: U]  #<br>#
+(** [G @@ S ⊢# t: T]    #<br>#
+    [G @@ S ⊢# T <: U]  #<br>#
     [―――――――――――――] #<br>#
-    [G ⊢# t: U]        *)
-| ty_sub_t : forall G t T U,
-    G ⊢# t : T ->
-    G ⊢# T <: U ->
-    G ⊢# t : U
-where "G '⊢#' t ':' T" := (ty_trm_t G t T)
+    [G @@ S ⊢# t: U]        *)
+| ty_sub_t : forall G S t T U,
+    G @@ S ⊢# t : T ->
+    G @@ S ⊢# T <: U ->
+    G @@ S ⊢# t : U
 
-(** *** Tight subtyping [G ⊢# T <: U] *)
-with subtyp_t : ctx -> typ -> typ -> Prop :=
+| ty_ref_intro : forall G S x T,
+    G @@ S ⊢# trm_var (avar_f x) : T ->
+    G @@ S ⊢# (trm_ref (avar_f x) T) : typ_ref T
 
-(** [G ⊢# T <: top] *)
-| subtyp_top_t: forall G T,
-    G ⊢# T <: typ_top
+| ty_ref_elim : forall G S x T,
+    G @@ S ⊢# trm_var (avar_f x) : typ_ref T ->
+    G @@ S ⊢# trm_deref (avar_f x) : T
 
-(** [G ⊢# bot <: T] *)
-| subtyp_bot_t: forall G T,
-    G ⊢# typ_bot <: T
+| ty_asgn : forall G S x y T,
+    G @@ S ⊢# trm_var (avar_f x) : typ_ref T ->
+    G @@ S ⊢# trm_var (avar_f y) : T ->
+    G @@ S ⊢# trm_asg (avar_f x) (avar_f y) : T
+where "G '@@' S '⊢#' t ':' T" := (ty_trm_t G S t T)
 
-(** [G ⊢# T <: T] *)
-| subtyp_refl_t: forall G T,
-    G ⊢# T <: T
+(** *** Tight subtyping [G @@ S ⊢# T <: U] *)
+with subtyp_t : ctx -> sigma -> typ -> typ -> Prop :=
 
-(** [G ⊢# S <: T]     #<br>#
-    [G ⊢# T <: U]     #<br>#
+(** [G @@ S ⊢# T <: top] *)
+| subtyp_top_t: forall G S T,
+    G @@ S ⊢# T <: typ_top
+
+(** [G @@ S ⊢# bot <: T] *)
+| subtyp_bot_t: forall G S T,
+    G @@ S ⊢# typ_bot <: T
+
+(** [G @@ S ⊢# T <: T] *)
+| subtyp_refl_t: forall G S T,
+    G @@ S ⊢# T <: T
+
+(** [G @@ S ⊢# S <: T]     #<br>#
+    [G @@ S ⊢# T <: U]     #<br>#
     [―――――――――――――]    #<br>#
-    [G ⊢# S <: U]         *)
-| subtyp_trans_t: forall G S T U,
-    G ⊢# S <: T ->
-    G ⊢# T <: U ->
-    G ⊢# S <: U
+    [G @@ S ⊢# S <: U]         *)
+| subtyp_trans_t: forall G S T U V,
+    G @@ S ⊢# T <: U ->
+    G @@ S ⊢# U <: V ->
+    G @@ S ⊢# T <: V
 
-(** [G ⊢# T /\ U <: T] *)
-| subtyp_and11_t: forall G T U,
-    G ⊢# typ_and T U <: T
+(** [G @@ S ⊢# T /\ U <: T] *)
+| subtyp_and11_t: forall G S T U,
+    G @@ S ⊢# typ_and T U <: T
 
-(** [G ⊢# T /\ U <: U] *)
-| subtyp_and12_t: forall G T U,
-    G ⊢# typ_and T U <: U
+(** [G @@ S ⊢# T /\ U <: U] *)
+| subtyp_and12_t: forall G S T U,
+    G @@ S ⊢# typ_and T U <: U
 
-(** [G ⊢# S <: T]       #<br>#
-    [G ⊢# S <: U]       #<br>#
+(** [G @@ S ⊢# S <: T]       #<br>#
+    [G @@ S ⊢# S <: U]       #<br>#
     [――――――――――――――――]   #<br>#
-    [G ⊢# S <: T /\ U]       *)
-| subtyp_and2_t: forall G S T U,
-    G ⊢# S <: T ->
-    G ⊢# S <: U ->
-    G ⊢# S <: typ_and T U
+    [G @@ S ⊢# S <: T /\ U]       *)
+| subtyp_and2_t: forall G S T U V,
+    G @@ S ⊢# T <: U ->
+    G @@ S ⊢# T <: V ->
+    G @@ S ⊢# T <: typ_and U V
 
-(** [G ⊢# T <: U]           #<br>#
+(** [G @@ S ⊢# T <: U]           #<br>#
     [――――――――――――――――――――――] #<br>#
-    [G ⊢# {a: T} <: {a: U}]     *)
-| subtyp_fld_t: forall G a T U,
-    G ⊢# T <: U ->
-    G ⊢# typ_rcd (dec_trm a T) <: typ_rcd (dec_trm a U)
+    [G @@ S ⊢# {a: T} <: {a: U}]     *)
+| subtyp_fld_t: forall G S a T U,
+    G @@ S ⊢# T <: U ->
+    G @@ S ⊢# typ_rcd (dec_trm a T) <: typ_rcd (dec_trm a U)
 
-(** [G ⊢# S2 <: S1]                   #<br>#
-    [G ⊢# T1 <: T2]                   #<br>#
+(** [G @@ S ⊢# S2 <: S1]                   #<br>#
+    [G @@ S ⊢# T1 <: T2]                   #<br>#
     [――――――――――――――――――――――――――――――――] #<br>#
-    [G ⊢# {A: S1..T1} <: {A: S2..T2}]     *)
-| subtyp_typ_t: forall G A S1 T1 S2 T2,
-    G ⊢# S2 <: S1 ->
-    G ⊢# T1 <: T2 ->
-    G ⊢# typ_rcd (dec_typ A S1 T1) <: typ_rcd (dec_typ A S2 T2)
+    [G @@ S ⊢# {A: S1..T1} <: {A: S2..T2}]     *)
+| subtyp_typ_t: forall G S A S1 T1 S2 T2,
+    G @@ S ⊢# S2 <: S1 ->
+    G @@ S ⊢# T1 <: T2 ->
+    G @@ S ⊢# typ_rcd (dec_typ A S1 T1) <: typ_rcd (dec_typ A S2 T2)
 
-(** [G ⊢! x: {A: T..T}] #<br>#
+(** [G @@ S ⊢! x: {A: T..T}] #<br>#
     [――――――――――――――――――] #<br>#
-    [G ⊢# T <: x.A]         *)
-| subtyp_sel2_t: forall G x A T,
-    G ⊢! trm_var (avar_f x) : typ_rcd (dec_typ A T T) ->
-    G ⊢# T <: typ_sel (avar_f x) A
+    [G @@ S ⊢# T <: x.A]         *)
+| subtyp_sel2_t: forall G S x A T,
+    G @@ S ⊢! trm_var (avar_f x) : typ_rcd (dec_typ A T T) ->
+    G @@ S ⊢# T <: typ_sel (avar_f x) A
 
-(** [G ⊢! x: {A: T..T}] #<br>#
+(** [G @@ S ⊢! x: {A: T..T}] #<br>#
     [――――――――――――――――――] #<br>#
-    [G ⊢# x.A <: T]         *)
-| subtyp_sel1_t: forall G x A T,
-    G ⊢! trm_var (avar_f x) : typ_rcd (dec_typ A T T) ->
-    G ⊢# typ_sel (avar_f x) A <: T
+    [G @@ S ⊢# x.A <: T]         *)
+| subtyp_sel1_t: forall G S x A T,
+    G @@ S ⊢! trm_var (avar_f x) : typ_rcd (dec_typ A T T) ->
+    G @@ S ⊢# typ_sel (avar_f x) A <: T
 
-(** [G ⊢# S2 <: S1]                #<br>#
-    [G, x: S2 ⊢ T1^x <: T2^x]       #<br>#
+(** [G @@ S ⊢# S2 <: S1]                #<br>#
+    [G, x: S2 @@ S ⊢ T1^x <: T2^x]       #<br>#
     [x fresh]                       #<br>#
     [――――――――――――――――――――――――]      #<br>#
-    [G ⊢# forall(S1)T1 <: forall(S2)T2]          *)
-| subtyp_all_t: forall L G S1 T1 S2 T2,
-    G ⊢# S2 <: S1 ->
+    [G @@ S ⊢# forall(S1)T1 <: forall(S2)T2]          *)
+| subtyp_all_t: forall L G S S1 T1 S2 T2,
+    G @@ S ⊢# S2 <: S1 ->
     (forall x, x \notin L ->
-       G & x ~ S2 ⊢ open_typ x T1 <: open_typ x T2) ->
-    G ⊢# typ_all S1 T1 <: typ_all S2 T2
-where "G '⊢#' T '<:' U" := (subtyp_t G T U).
+       G & x ~ S2 @@ S ⊢ open_typ x T1 <: open_typ x T2) ->
+    G @@ S ⊢# typ_all S1 T1 <: typ_all S2 T2
+where "G '@@' S '⊢#' T '<:' U" := (subtyp_t G S T U).
 
 Hint Constructors ty_trm_t subtyp_t.
 
@@ -204,12 +221,12 @@ Combined Scheme ts_t_mutind from ts_ty_trm_t_mut, ts_subtyp_t.
 
 (** Tight typing implies general typing. *)
 Lemma tight_to_general:
-  (forall G t T,
-     G ⊢# t : T ->
-     G ⊢ t : T) /\
-  (forall G S U,
-     G ⊢# S <: U ->
-     G ⊢ S <: U).
+  (forall G S t T,
+     G @@ S ⊢# t : T ->
+     G @@ S ⊢ t : T) /\
+  (forall G S T U,
+     G @@ S ⊢# T <: U ->
+     G @@ S ⊢ T <: U).
 Proof.
   apply ts_t_mutind; intros; subst; eauto using precise_to_general.
 Qed.
